src/impl/TLS13.Impl.Client.Driver.fst
@@ -2249,6 +2249,8 @@ fn driver_process_buffered_network_bytes_once
     assert (A.pts_to_mask raw_prefix_array #1.0R raw_prefix_mask_after (fun _ -> True));
   assert (pure (forall (i:nat). i < Seq.length raw_prefix_mask_after ==>
     Some? (Seq.index raw_prefix_mask_after i)));
+  assert (pure (forall (i:nat). i < Seq.length raw_prefix_mask_after ==>
+    Seq.index raw_prefix_mask_after i == Some (Seq.index (Ghost.reveal 'old_raw) i)));
   rewrite
     (A.pts_to_mask raw_prefix_array #1.0R raw_prefix_mask_after (fun _ -> True))
     as
@@ -2272,6 +2274,8 @@ fn driver_process_buffered_network_bytes_once
      (0 <= i /\ i < SZ.v buffered_len /\ True))));
   assert (pure (forall (i:nat). i < Seq.length raw_joined_mask ==>
     Some? (Seq.index raw_joined_mask i)));
+  assert (pure (forall (i:nat). i < Seq.length raw_joined_mask ==>
+    Seq.index raw_joined_mask i == Some (Seq.index (Ghost.reveal 'old_raw) i)));
   A.from_mask raw;
   with raw_bytes.
     assert (pts_to raw raw_bytes);
