src/impl/TLS13.Impl.Server.Auth.fsti
@@ -92,12 +92,12 @@ fn process_sign_certificate_verify
                  (match 'st0.CS.cs_model.CS.model_handshake.CS.hs_server_selection with
                   | Some selection ->
                     selection.CS.server_selected_signature_scheme ==
-                      T.RsaPssRsaeSha256 /\
+                      T.Rsa_pss_rsae_sha256 /\
                     selection.CS.server_selected_credential ==
                       Ghost.reveal 'credential_identity /\
                     CS.signature_scheme_offered
                       'st0.CS.cs_model.CS.model_config.CS.config_signature_schemes
-                      T.RsaPssRsaeSha256
+                      T.Rsa_pss_rsae_sha256
                   | None -> False))
   returns resp:ST.server_response
   ensures exists* st1 network_out_bytes app_out_bytes.
