src/spec/TLS13.ConnectionState.Lemmas.fst
@@ -375,11 +375,11 @@ let lemma_legal_tls_message_stable_client_x25519_key_share_projection
       hs0.hs_keys.ks_shared_secret);
     assert (client_x25519_key_share_projection st1);
     assert (client_x25519_key_share_projection_stable_control st1.cs_model.model_control)
-  | M.TlsAlert T.CloseNotify, ControlApplicationData ->
+  | M.TlsAlert T.Close_notify, ControlApplicationData ->
     assert (st1.cs_model.model_handshake == hs0);
     assert (client_x25519_key_share_projection st1);
     assert (client_x25519_key_share_projection_stable_control st1.cs_model.model_control)
-  | M.TlsAlert T.CloseNotify, ControlClosing ->
+  | M.TlsAlert T.Close_notify, ControlClosing ->
     (match msg.CL.message_direction with
      | CL.Received ->
        assert (st1.cs_model.model_handshake == hs0);
@@ -485,11 +485,11 @@ let lemma_legal_tls_message_stable_server_x25519_key_share_projection
       hs0.hs_keys.ks_shared_secret);
     assert (server_x25519_key_share_projection st1);
     assert (server_x25519_key_share_projection_stable_control st1.cs_model.model_control)
-  | M.TlsAlert T.CloseNotify, ControlApplicationData ->
+  | M.TlsAlert T.Close_notify, ControlApplicationData ->
     assert (st1.cs_model.model_handshake == hs0);
     assert (server_x25519_key_share_projection st1);
     assert (server_x25519_key_share_projection_stable_control st1.cs_model.model_control)
-  | M.TlsAlert T.CloseNotify, ControlClosing ->
+  | M.TlsAlert T.Close_notify, ControlClosing ->
     (match msg.CL.message_direction with
      | CL.Received ->
        assert (st1.cs_model.model_handshake == hs0);
@@ -1582,9 +1582,9 @@ let lemma_connection_delta_client_x25519_reachable_shape
              | M.TlsIgnoredPostHandshake _, CL.Received, ControlApplicationData
              | M.TlsKeyUpdate _, CL.Received, ControlApplicationData
              | M.TlsKeyUpdate M.UpdateNotRequested, CL.Sent, ControlApplicationData
-             | M.TlsAlert T.CloseNotify, CL.Sent, ControlApplicationData
-             | M.TlsAlert T.CloseNotify, CL.Received, ControlApplicationData
-             | M.TlsAlert T.CloseNotify, CL.Received, ControlClosing
+             | M.TlsAlert T.Close_notify, CL.Sent, ControlApplicationData
+             | M.TlsAlert T.Close_notify, CL.Received, ControlApplicationData
+             | M.TlsAlert T.Close_notify, CL.Received, ControlClosing
              | M.TlsAlert _, _, _
              | M.TlsChangeCipherSpec, _, ControlHandshaking _ ->
                assert (step_tls_message
@@ -1776,9 +1776,9 @@ let lemma_connection_delta_server_x25519_reachable_shape
              | M.TlsIgnoredPostHandshake _, CL.Received, ControlApplicationData
              | M.TlsKeyUpdate _, CL.Received, ControlApplicationData
              | M.TlsKeyUpdate M.UpdateNotRequested, CL.Sent, ControlApplicationData
-             | M.TlsAlert T.CloseNotify, CL.Sent, ControlApplicationData
-             | M.TlsAlert T.CloseNotify, CL.Received, ControlApplicationData
-             | M.TlsAlert T.CloseNotify, CL.Received, ControlClosing
+             | M.TlsAlert T.Close_notify, CL.Sent, ControlApplicationData
+             | M.TlsAlert T.Close_notify, CL.Received, ControlApplicationData
+             | M.TlsAlert T.Close_notify, CL.Received, ControlClosing
              | M.TlsAlert _, _, _
              | M.TlsChangeCipherSpec, _, ControlHandshaking _ ->
                assert (step_tls_message
@@ -2141,8 +2141,8 @@ let lemma_step_model_server_handshake_write_key_reachable_shape
       | M.TlsApplicationData _, _, ControlApplicationData
       | M.TlsIgnoredPostHandshake _, _, ControlApplicationData
       | M.TlsKeyUpdate _, _, ControlApplicationData
-      | M.TlsAlert T.CloseNotify, _, ControlApplicationData
-      | M.TlsAlert T.CloseNotify, _, ControlClosing ->
+      | M.TlsAlert T.Close_notify, _, ControlApplicationData
+      | M.TlsAlert T.Close_notify, _, ControlClosing ->
         ()
       | M.TlsAlert _, _,
         _ ->
@@ -2571,15 +2571,15 @@ let lemma_step_model_application_record_epoch_reachable_shape_for_role
                     model.model_record.record_read);
             assert (model'.model_record.record_write.R.epoch == R.Application);
             assert (client_application_record_epoch_link model')
-          | M.TlsAlert T.CloseNotify, CL.Sent, ControlApplicationData ->
+          | M.TlsAlert T.Close_notify, CL.Sent, ControlApplicationData ->
             assert (client_application_record_epoch_link model);
             assert (model'.model_record.record_read ==
                     model.model_record.record_read);
             assert (model'.model_record.record_write.R.epoch ==
                     (R.next_seq model.model_record.record_write).R.epoch);
             assert (client_application_record_epoch_link model')
-          | M.TlsAlert T.CloseNotify, CL.Received, ControlApplicationData
-          | M.TlsAlert T.CloseNotify, CL.Received, ControlClosing ->
+          | M.TlsAlert T.Close_notify, CL.Received, ControlApplicationData
+          | M.TlsAlert T.Close_notify, CL.Received, ControlClosing ->
             assert (client_application_record_epoch_link model);
             assert (model'.model_record.record_write ==
                     model.model_record.record_write);
@@ -2742,15 +2742,15 @@ let lemma_step_model_application_record_epoch_reachable_shape_for_role
             assert (model'.model_record.record_read.R.epoch ==
                     (R.next_seq model.model_record.record_read).R.epoch);
             assert (server_application_record_epoch_link model')
-          | M.TlsAlert T.CloseNotify, CL.Sent, ControlApplicationData ->
+          | M.TlsAlert T.Close_notify, CL.Sent, ControlApplicationData ->
             assert (server_application_record_epoch_link model);
             assert (model'.model_record.record_read ==
                     model.model_record.record_read);
             assert (model'.model_record.record_write.R.epoch ==
                     (R.next_seq model.model_record.record_write).R.epoch);
             assert (server_application_record_epoch_link model')
-          | M.TlsAlert T.CloseNotify, CL.Received, ControlApplicationData
-          | M.TlsAlert T.CloseNotify, CL.Received, ControlClosing ->
+          | M.TlsAlert T.Close_notify, CL.Received, ControlApplicationData
+          | M.TlsAlert T.Close_notify, CL.Received, ControlClosing ->
             assert (server_application_record_epoch_link model);
             assert (model'.model_record.record_write ==
                     model.model_record.record_write);
@@ -4498,7 +4498,7 @@ let lemma_step_model_record_keys_consistent
        lemma_record_read_keys_next_seq
          model0.model_handshake.hs_keys
          model0.model_record.record_read
-     | CL.Received, M.TlsAlert T.CloseNotify ->
+     | CL.Received, M.TlsAlert T.Close_notify ->
        (match model1.model_control with
         | ControlFailed _ -> ()
         | _ ->
@@ -4508,7 +4508,7 @@ let lemma_step_model_record_keys_consistent
           lemma_record_read_keys_next_seq
             model0.model_handshake.hs_keys
             model0.model_record.record_read)
-     | CL.Sent, M.TlsAlert T.CloseNotify ->
+     | CL.Sent, M.TlsAlert T.Close_notify ->
        (match model1.model_control with
         | ControlFailed _ -> ()
         | _ ->
@@ -4659,7 +4659,7 @@ let lemma_step_model_record_keys_consistent_for_role
            model0.model_control
            model0.model_handshake.hs_keys
            model0.model_record.record_write
-       | M.TlsAlert T.CloseNotify ->
+       | M.TlsAlert T.Close_notify ->
          (match model0.model_control with
           | ControlApplicationData ->
             assert (model1.model_handshake.hs_keys == model0.model_handshake.hs_keys);
@@ -4909,7 +4909,7 @@ let lemma_step_model_record_layer_delta
                projected_next_seq
                  (projected_record_layer_state_of_record model0.model_record).projected_read });
        assert (model_record_layer_delta model0 ev model1)
-     | CL.Received, M.TlsAlert T.CloseNotify ->
+     | CL.Received, M.TlsAlert T.Close_notify ->
        (match model0.model_control with
         | ControlApplicationData
         | ControlClosing ->
@@ -4929,9 +4929,9 @@ let lemma_step_model_record_layer_delta
                     (projected_record_layer_state_of_record model0.model_record).projected_read });
           assert (model_record_layer_delta model0 ev model1)
         | _ ->
-          assert (model1.model_control == ControlFailed (T.AlertError T.CloseNotify));
+          assert (model1.model_control == ControlFailed (T.AlertError T.Close_notify));
           assert (model_record_layer_delta model0 ev model1))
-     | CL.Sent, M.TlsAlert T.CloseNotify ->
+     | CL.Sent, M.TlsAlert T.Close_notify ->
        (match model0.model_control with
         | ControlApplicationData ->
           assert (model1.model_record == {
@@ -4950,7 +4950,7 @@ let lemma_step_model_record_layer_delta
                     (projected_record_layer_state_of_record model0.model_record).projected_write });
           assert (model_record_layer_delta model0 ev model1)
         | _ ->
-          assert (model1.model_control == ControlFailed (T.AlertError T.CloseNotify));
+          assert (model1.model_control == ControlFailed (T.AlertError T.Close_notify));
           assert (model_record_layer_delta model0 ev model1))
      | _, _ ->
        assert (model1.model_record == model0.model_record);
@@ -5521,9 +5521,9 @@ let lemma_raw_records_exactly_single_serialized
 let lemma_raw_application_data_record_exactly
   (fragment:B.bytes{B.length fragment <= 16640})
   : Lemma
-      (raw_records_exactly (W.serialize_record T.ApplicationData fragment) T.ApplicationData 1)
+      (raw_records_exactly (W.serialize_record T.Application_data fragment) T.Application_data 1)
 =
-  lemma_raw_records_exactly_single_serialized T.ApplicationData fragment
+  lemma_raw_records_exactly_single_serialized T.Application_data fragment
 
 let lemma_parse_record_full_raw_records_exactly
   (raw:B.bytes)
@@ -5559,13 +5559,13 @@ let lemma_sent_single_protected_message_seal_intro
   (ciphertext:B.bytes)
   : Lemma
       (requires
-        W.parse_record raw == Some (T.ApplicationData, ciphertext, B.length raw) /\
+        W.parse_record raw == Some (T.Application_data, ciphertext, B.length raw) /\
         Seq.equal aad (record_header_aad raw) /\
         R.seal
           model.model_record.record_write
           aad
           {
-            R.content_type = T.ApplicationData;
+            R.content_type = T.Application_data;
             R.fragment = sent_tls_inner_plaintext_fragment msg;
           } ==
           Some (ciphertext, R.next_seq model.model_record.record_write))
@@ -5573,12 +5573,12 @@ let lemma_sent_single_protected_message_seal_intro
 =
   Seq.lemma_eq_elim aad (record_header_aad raw);
   assert (exists ciphertext'.
-    W.parse_record raw == Some (T.ApplicationData, ciphertext', B.length raw) /\
+    W.parse_record raw == Some (T.Application_data, ciphertext', B.length raw) /\
     R.seal
       model.model_record.record_write
       (record_header_aad raw)
       {
-        R.content_type = T.ApplicationData;
+        R.content_type = T.Application_data;
         R.fragment = sent_tls_inner_plaintext_fragment msg;
       } ==
       Some (ciphertext', R.next_seq model.model_record.record_write))
@@ -5604,14 +5604,14 @@ let lemma_sent_event_seal_projection_intro
       (requires
         network_message_is_cleartext CL.Sent msg == false /\
         protected_record_count CL.Sent msg == 1 /\
-        W.parse_record raw == Some (T.ApplicationData, ciphertext, B.length raw) /\
+        W.parse_record raw == Some (T.Application_data, ciphertext, B.length raw) /\
         Seq.equal aad (record_header_aad raw) /\
         Seq.equal plaintext (sent_tls_inner_plaintext_fragment msg) /\
         R.seal
           model.model_record.record_write
           aad
           {
-            R.content_type = T.ApplicationData;
+            R.content_type = T.Application_data;
             R.fragment = plaintext;
           } ==
           Some (ciphertext, R.next_seq model.model_record.record_write))
@@ -5636,10 +5636,10 @@ let lemma_network_message_raw_delta_legal_protected_single_parse_record
         network_message_is_cleartext msg.CL.message_direction msg.CL.message_value == false /\
         protected_record_count msg.CL.message_direction msg.CL.message_value == 1)
       (ensures exists fragment.
-        W.parse_record raw == Some (T.ApplicationData, fragment, B.length raw))
+        W.parse_record raw == Some (T.Application_data, fragment, B.length raw))
 =
-  assert (raw_records_exactly raw T.ApplicationData 1);
-  lemma_raw_records_exactly_one_parse_record raw T.ApplicationData
+  assert (raw_records_exactly raw T.Application_data 1);
+  lemma_raw_records_exactly_one_parse_record raw T.Application_data
 
 let lemma_network_message_raw_delta_legal_protected_parse_prefix
   (model:connection_model)
@@ -5650,14 +5650,14 @@ let lemma_network_message_raw_delta_legal_protected_parse_prefix
         network_message_raw_delta_legal model msg raw /\
         network_message_is_cleartext msg.CL.message_direction msg.CL.message_value == false)
       (ensures exists fragment. exists (consumed:nat).
-        W.parse_record raw == Some (T.ApplicationData, fragment, consumed) /\
+        W.parse_record raw == Some (T.Application_data, fragment, consumed) /\
         consumed > 0 /\
         consumed <= B.length raw)
 =
   lemma_protected_record_count_positive msg.CL.message_direction msg.CL.message_value;
   lemma_raw_records_exactly_nonempty_parse_record
     raw
-    T.ApplicationData
+    T.Application_data
     (protected_record_count msg.CL.message_direction msg.CL.message_value)
 
 let lemma_network_message_raw_delta_legal_protected_decompose
@@ -5669,7 +5669,7 @@ let lemma_network_message_raw_delta_legal_protected_decompose
         network_message_raw_delta_legal model msg raw /\
         network_message_is_cleartext msg.CL.message_direction msg.CL.message_value == false)
       (ensures exists fragment. exists (consumed:nat).
-        W.parse_record raw == Some (T.ApplicationData, fragment, consumed) /\
+        W.parse_record raw == Some (T.Application_data, fragment, consumed) /\
         consumed > 0 /\
         consumed <= B.length raw /\
         (let rest = Seq.slice raw consumed (B.length raw) in
@@ -5678,12 +5678,12 @@ let lemma_network_message_raw_delta_legal_protected_decompose
          Seq.equal tail.CL.residual B.empty /\
          length tail.CL.values ==
            protected_record_count msg.CL.message_direction msg.CL.message_value - 1 /\
-         all_records_outer_type T.ApplicationData tail.CL.values))
+         all_records_outer_type T.Application_data tail.CL.values))
 =
   lemma_protected_record_count_positive msg.CL.message_direction msg.CL.message_value;
   lemma_raw_records_exactly_nonempty_decompose
     raw
-    T.ApplicationData
+    T.Application_data
     (protected_record_count msg.CL.message_direction msg.CL.message_value)
 
 let lemma_network_message_raw_delta_legal_protected_decompose_prefix
@@ -5695,18 +5695,18 @@ let lemma_network_message_raw_delta_legal_protected_decompose_prefix
         network_message_raw_delta_legal model msg raw /\
         network_message_is_cleartext msg.CL.message_direction msg.CL.message_value == false)
       (ensures exists fragment. exists (consumed:nat).
-        W.parse_record raw == Some (T.ApplicationData, fragment, consumed) /\
+        W.parse_record raw == Some (T.Application_data, fragment, consumed) /\
         consumed > 0 /\
         consumed <= B.length raw /\
         raw_records_exactly
           (Seq.slice raw consumed (B.length raw))
-          T.ApplicationData
+          T.Application_data
           (protected_record_count msg.CL.message_direction msg.CL.message_value - 1))
 =
   lemma_protected_record_count_positive msg.CL.message_direction msg.CL.message_value;
   lemma_raw_records_exactly_nonempty_decompose_prefix
     raw
-    T.ApplicationData
+    T.Application_data
     (protected_record_count msg.CL.message_direction msg.CL.message_value)
 
 let lemma_network_message_raw_delta_legal_protected_segmented
@@ -5719,12 +5719,12 @@ let lemma_network_message_raw_delta_legal_protected_segmented
         network_message_is_cleartext msg.CL.message_direction msg.CL.message_value == false)
       (ensures raw_records_segmented
         raw
-        T.ApplicationData
+        T.Application_data
         (protected_record_count msg.CL.message_direction msg.CL.message_value))
 =
   lemma_raw_records_exactly_segmented
     raw
-    T.ApplicationData
+    T.Application_data
     (protected_record_count msg.CL.message_direction msg.CL.message_value)
 
 let lemma_event_raw_delta_legal_protected_single_parse_record
@@ -5750,7 +5750,7 @@ let lemma_event_raw_delta_legal_protected_single_parse_record
         lemma_network_message_raw_delta_legal_protected_single_parse_record model msg raw_received;
         assert (exists fragment.
           W.parse_record raw_received ==
-            Some (T.ApplicationData, fragment, B.length raw_received));
+            Some (T.Application_data, fragment, B.length raw_received));
         W.lemma_parse_record_implies_parse_record_wire raw_received
     else ()
 
@@ -5776,7 +5776,7 @@ let lemma_event_raw_delta_legal_protected_parse_prefix
         lemma_network_message_raw_delta_legal_protected_parse_prefix model msg raw_received;
         assert (exists fragment. exists (consumed:nat).
           W.parse_record raw_received ==
-            Some (T.ApplicationData, fragment, consumed) /\
+            Some (T.Application_data, fragment, consumed) /\
           consumed > 0 /\
           consumed <= B.length raw_received);
         W.lemma_parse_record_implies_parse_record_wire raw_received
@@ -5803,12 +5803,12 @@ let lemma_event_raw_delta_legal_protected_decompose_prefix
         lemma_network_message_raw_delta_legal_protected_decompose_prefix model msg raw_received;
         assert (exists fragment. exists (consumed:nat).
           W.parse_record raw_received ==
-            Some (T.ApplicationData, fragment, consumed) /\
+            Some (T.Application_data, fragment, consumed) /\
           consumed > 0 /\
           consumed <= B.length raw_received /\
           raw_records_exactly
             (Seq.slice raw_received consumed (B.length raw_received))
-            T.ApplicationData
+            T.Application_data
             (protected_record_count msg.CL.message_direction msg.CL.message_value - 1));
         W.lemma_parse_record_implies_parse_record_wire raw_received
 
