src/spec/TLS13.ConnectionState.Lemmas.fsti
@@ -410,14 +410,14 @@ val lemma_sent_event_seal_projection_intro
       (requires
         network_message_is_cleartext CL.Sent msg == false /\
         protected_record_count CL.Sent msg == 1 /\
-        W.parse_record raw == Some (T.ApplicationData, ciphertext, B.length raw) /\
+        W.parse_record raw == Some (T.Application_data, ciphertext, B.length raw) /\
         Seq.equal aad (record_header_aad raw) /\
         Seq.equal plaintext (sent_tls_inner_plaintext_fragment msg) /\
         R.seal
           model.model_record.record_write
           aad
           {
-            R.content_type = T.ApplicationData;
+            R.content_type = T.Application_data;
             R.fragment = plaintext;
           } ==
           Some (ciphertext, R.next_seq model.model_record.record_write))
